finishing porting the CDCL part of IsaSAT

Weidenbach_Book/IsaSAT_CDCL.thy
@@ -82,16 +82,26 @@ where
 definition (in isasat_input_ops) find_unassigned_lit_wl_D_heur
   :: \<open>twl_st_wl_heur \<Rightarrow> (twl_st_wl_heur \<times> nat literal option) nres\<close>
 where
-  \<open>find_unassigned_lit_wl_D_heur = (\<lambda>(M, N, U, D, WS, Q, vm, \<phi>, clvls). do {
+  \<open>find_unassigned_lit_wl_D_heur = (\<lambda>(M, N, D, WS, Q, vm, \<phi>, clvls). do {
       ASSERT(vm \<in> vmtf M \<and> phase_saving \<phi>);
       ((M, vm), L) \<leftarrow> find_undefined_atm M vm;
       L \<leftarrow> lit_of_found_atm \<phi> L;
-      RETURN ((M, N, U, D, WS, Q, vm, \<phi>, clvls), L)
+      RETURN ((M, N, D, WS, Q, vm, \<phi>, clvls), L)
     })\<close>
 
+definition find_unassigned_lit_wl_D_heur_pre where
+  \<open>find_unassigned_lit_wl_D_heur_pre S \<longleftrightarrow>
+    (
+      \<exists>T U.
+        (S, T) \<in> state_wl_l None \<and>
+        (T, U) \<in> twl_st_l None \<and>
+        twl_struct_invs U \<and>
+        literals_are_\<L>\<^sub>i\<^sub>n S \<and>
+        get_conflict_wl S = None
+    )\<close>
 lemma find_unassigned_lit_wl_D'_find_unassigned_lit_wl_D:
   \<open>(find_unassigned_lit_wl_D_heur, find_unassigned_lit_wl_D) \<in>
-     [\<lambda>S. twl_struct_invs (twl_st_of_wl None S) \<and> literals_are_\<L>\<^sub>i\<^sub>n S \<and> get_conflict_wl S = None]\<^sub>f
+     [find_unassigned_lit_wl_D_heur_pre]\<^sub>f
     twl_st_heur \<rightarrow> \<langle>{((T, L), (T', L')). (T, T') \<in> twl_st_heur \<and> L = L' \<and>
          (L \<noteq> None \<longrightarrow> undefined_lit (get_trail_wl T') (the L) \<and> the L \<in># \<L>\<^sub>a\<^sub>l\<^sub>l) \<and>
          get_conflict_wl T' = None}\<rangle>nres_rel\<close>
@@ -104,24 +114,33 @@ proof -
   have ID_R: \<open>Id \<times>\<^sub>r \<langle>Id\<rangle>option_rel = Id\<close>
     by auto
   have atms: \<open>atms_of \<L>\<^sub>a\<^sub>l\<^sub>l =
-         atms_of_ms ((\<lambda>x. mset (watched_l x) + mset (unwatched_l x)) ` set (take U (tl N))) \<union>
-         atms_of_mm NE\<close>
-      if inv: \<open>twl_struct_invs (twl_st_of_wl None (M, N, U, D, NE, UE, WS, Q))\<close> and
-        \<A>\<^sub>i\<^sub>n: \<open>literals_are_\<L>\<^sub>i\<^sub>n (M, N, U, D, NE, UE, WS, Q)\<close> and
-        confl: \<open>get_conflict_wl (M, N, U, D, NE, UE, WS, Q) = None\<close>
-      for M N U D NE UE WS Q
+         atms_of_mm (mset `# init_clss_lf N) \<union>
+         atms_of_mm NE \<and> D = None\<close>
+      if inv: \<open>find_unassigned_lit_wl_D_heur_pre (M, N, D, NE, UE, WS, Q)\<close>
+      for M N D NE UE WS Q
   proof -
-    have \<open>cdcl\<^sub>W_restart_mset.no_strange_atm
-            (state\<^sub>W_of (twl_st_of_wl None (M, N, U, D, NE, UE, WS, Q)))\<close> and
-        unit: \<open>entailed_clss_inv (twl_st_of_wl None (M, N, U, D, NE, UE, WS, Q))\<close>
+    obtain T U where
+      S_T: \<open>((M, N, D, NE, UE, WS, Q), T) \<in> state_wl_l None\<close> and
+      T_U: \<open>(T, U) \<in> twl_st_l None\<close> and
+      inv: \<open>twl_struct_invs U\<close> and
+      \<A>\<^sub>i\<^sub>n : \<open>literals_are_\<L>\<^sub>i\<^sub>n (M, N, D, NE, UE, WS, Q)\<close> and
+      confl: \<open>get_conflict_wl (M, N, D, NE, UE, WS, Q) = None\<close>
+      using inv unfolding find_unassigned_lit_wl_D_heur_pre_def
+       apply - apply normalize_goal+
+       by blast
+      
+    have \<open>cdcl\<^sub>W_restart_mset.no_strange_atm (state\<^sub>W_of U)\<close> and
+        unit: \<open>entailed_clss_inv U\<close>
       using inv unfolding twl_struct_invs_def cdcl\<^sub>W_restart_mset.cdcl\<^sub>W_all_struct_inv_def
       by fast+
     then show ?thesis
-      using \<A>\<^sub>i\<^sub>n unfolding is_\<L>\<^sub>a\<^sub>l\<^sub>l_alt_def
-      by (auto simp: cdcl\<^sub>W_restart_mset.no_strange_atm_def
+      using \<A>\<^sub>i\<^sub>n confl S_T T_U unfolding is_\<L>\<^sub>a\<^sub>l\<^sub>l_alt_def state_wl_l_def twl_st_l_def apply -
+      by (subst (asm) all_clss_l_ran_m[symmetric], subst (asm) image_mset_union)
+        (auto simp: cdcl\<^sub>W_restart_mset.no_strange_atm_def entailed_clss_inv.simps
           mset_take_mset_drop_mset mset_take_mset_drop_mset'
           clauses_def simp del: entailed_clss_inv.simps)
   qed
+  
   have [dest]: \<open>(S, T) \<in> twl_st_heur \<Longrightarrow> \<phi> = get_phase_saver_heur S \<Longrightarrow> phase_saving \<phi>\<close> for S T \<phi>
     by (auto simp: twl_st_heur_def)
 
@@ -132,8 +151,8 @@ proof -
    apply clarify
    apply refine_vcg
    unfolding RETURN_RES_refine_iff
-   by (auto simp add: twl_st_heur_def atms in_\<L>\<^sub>a\<^sub>l\<^sub>l_atm_of_in_atms_of_iff Ball_def image_image
-       mset_take_mset_drop_mset'
+   by (auto simp add: twl_st_heur_def in_\<L>\<^sub>a\<^sub>l\<^sub>l_atm_of_in_atms_of_iff Ball_def image_image
+       mset_take_mset_drop_mset' atms
         simp del: twl_st_of_wl.simps dest!: atms)
 qed
 
@@ -235,8 +254,8 @@ lemmas find_unassigned_lit_wl_D_heur_hnr[sepref_fr_rules] =
    find_unassigned_lit_wl_D_code.refine[of \<A>\<^sub>i\<^sub>n, OF isasat_input_bounded_nempty_axioms]
 
 definition (in isasat_input_ops) decide_lit_wl_heur :: \<open>nat literal \<Rightarrow> twl_st_wl_heur \<Rightarrow> twl_st_wl_heur\<close> where
-  \<open>decide_lit_wl_heur = (\<lambda>L' (M, N, U, D, Q, W, vmtf, \<phi>, clvls, cach, lbd, outl, stats).
-      (Decided L' # M, N, U, D, {#- L'#}, W, vmtf, \<phi>, clvls, cach, lbd, outl, incr_decision stats))\<close>
+  \<open>decide_lit_wl_heur = (\<lambda>L' (M, N, D, Q, W, vmtf, \<phi>, clvls, cach, lbd, outl, stats).
+      (Decided L' # M, N, D, {#- L'#}, W, vmtf, \<phi>, clvls, cach, lbd, outl, incr_decision stats))\<close>
 
 sepref_thm decide_lit_wl_code
   is \<open>uncurry (RETURN oo decide_lit_wl_heur)\<close>
@@ -276,18 +295,23 @@ lemma decide_wl_or_skip_D_heur_decide_wl_or_skip_D:
   \<open>(decide_wl_or_skip_D_heur, decide_wl_or_skip_D) \<in> twl_st_heur \<rightarrow>\<^sub>f \<langle>bool_rel \<times>\<^sub>f twl_st_heur\<rangle> nres_rel\<close>
   supply [[goals_limit=1]]
   unfolding decide_wl_or_skip_D_heur_def decide_wl_or_skip_D_def decide_wl_or_skip_D_pre_def
-  decide_wl_or_skip_pre_def decide_l_or_skip_pre_def twl_st_of_wl.simps[symmetric]
+   decide_l_or_skip_pre_def twl_st_of_wl.simps[symmetric]
   apply (intro nres_relI frefI)
   apply (refine_vcg find_unassigned_lit_wl_D'_find_unassigned_lit_wl_D[THEN fref_to_Down])
-  subgoal by (auto simp del: twl_st_of.simps simp: twl_st_heur_def)
-  subgoal by (auto simp del: twl_st_of.simps simp: twl_st_heur_def)
-  subgoal by (auto simp del: twl_st_of.simps simp: twl_st_heur_def)
-  subgoal by (auto simp del: twl_st_of.simps simp: twl_st_heur_def)
-  subgoal by (auto simp del: twl_st_of.simps simp: twl_st_heur_def)
-  subgoal by (auto simp del: twl_st_of.simps simp: twl_st_heur_def)
-  subgoal by (auto simp del: twl_st_of.simps simp: twl_st_heur_def)
-  subgoal by (auto simp del: twl_st_of.simps)
-  subgoal by (auto simp del: twl_st_of.simps simp: twl_st_heur_def decide_lit_wl_heur_def
+  subgoal
+    unfolding decide_wl_or_skip_pre_def find_unassigned_lit_wl_D_heur_pre_def
+      decide_wl_or_skip_pre_def decide_l_or_skip_pre_def
+     apply normalize_goal+
+     apply (rule_tac x = xa in exI)
+     apply (rule_tac x = xb in exI)
+     apply auto
+     done
+  subgoal by (auto simp del: simp: twl_st_heur_def)
+  subgoal by (auto simp del: simp: twl_st_heur_def)
+  subgoal by (auto simp del: simp: twl_st_heur_def)
+  subgoal by (auto simp del: simp: twl_st_heur_def)
+  subgoal by (auto simp del: simp: twl_st_heur_def)
+  subgoal by (auto simp: twl_st_heur_def decide_lit_wl_heur_def
         decide_lit_wl_def counts_maximum_level_def intro!: vmtf_consD)
   done
 
@@ -338,7 +362,7 @@ sepref_register get_conflict_wl_is_None decide_wl_or_skip_D_heur skip_and_resolv
 
 (* TODO Move + kill get_conflict_wl_is_Nil *)
 definition (in -)get_conflict_wl_heur_is_Nil :: \<open>twl_st_wl_heur \<Rightarrow> bool\<close> where
-  \<open>get_conflict_wl_heur_is_Nil = (\<lambda>(M, N, U, D, NE, UE, Q, W). D \<noteq> None \<and> Multiset.is_empty (the D))\<close>
+  \<open>get_conflict_wl_heur_is_Nil = (\<lambda>(M, N, D, NE, UE, Q, W). D \<noteq> None \<and> Multiset.is_empty (the D))\<close>
 
 lemma get_conflict_wl_heur_is_Nil_alt_def:
   \<open>get_conflict_wl_heur_is_Nil S \<longleftrightarrow> get_conflict_wl_heur S = Some {#}\<close>
